README.md
@@ -2,9 +2,15 @@
 
 My study note for domain theory
 
-## Build:
+# Build:
 
 ```
 coq_makefile -f _CoqProject *.v -o Makefile
 make
+```
+
+# coqc:
+
+```
+$ coqc -Q . DschingisKhan theories/DomainTheory.v
 ```
